%2multibyte Version: 5.50.0.2960 CodePage: 936

\documentclass{article}
%%%%%%%%%%%%%%%%%%%%%%%%%%%%%%%%%%%%%%%%%%%%%%%%%%%%%%%%%%%%%%%%%%%%%%%%%%%%%%%%%%%%%%%%%%%%%%%%%%%%%%%%%%%%%%%%%%%%%%%%%%%%%%%%%%%%%%%%%%%%%%%%%%%%%%%%%%%%%%%%%%%%%%%%%%%%%%%%%%%%%%%%%%%%%%%%%%%%%%%%%%%%%%%%%%%%%%%%%%%%%%%%%%%%%%%%%%%%%%%%%%%%%%%%%%%%
\usepackage{amsfonts}

%TCIDATA{OutputFilter=LATEX.DLL}
%TCIDATA{Version=5.50.0.2960}
%TCIDATA{Codepage=936}
%TCIDATA{<META NAME="SaveForMode" CONTENT="1">}
%TCIDATA{BibliographyScheme=Manual}
%TCIDATA{Created=Saturday, July 11, 2020 15:08:03}
%TCIDATA{LastRevised=Monday, August 10, 2020 16:01:46}
%TCIDATA{<META NAME="GraphicsSave" CONTENT="32">}
%TCIDATA{<META NAME="DocumentShell" CONTENT="Standard LaTeX\Blank - Standard LaTeX Article">}
%TCIDATA{CSTFile=40 LaTeX article.cst}

\newtheorem{theorem}{Theorem}
\newtheorem{acknowledgement}[theorem]{Acknowledgement}
\newtheorem{algorithm}[theorem]{Algorithm}
\newtheorem{axiom}[theorem]{Axiom}
\newtheorem{case}[theorem]{Case}
\newtheorem{claim}[theorem]{Claim}
\newtheorem{conclusion}[theorem]{Conclusion}
\newtheorem{condition}[theorem]{Condition}
\newtheorem{conjecture}[theorem]{Conjecture}
\newtheorem{corollary}[theorem]{Corollary}
\newtheorem{criterion}[theorem]{Criterion}
\newtheorem{definition}[theorem]{Definition}
\newtheorem{example}[theorem]{Example}
\newtheorem{exercise}[theorem]{Exercise}
\newtheorem{lemma}[theorem]{Lemma}
\newtheorem{notation}[theorem]{Notation}
\newtheorem{problem}[theorem]{Problem}
\newtheorem{proposition}[theorem]{Proposition}
\newtheorem{remark}[theorem]{Remark}
\newtheorem{solution}[theorem]{Solution}
\newtheorem{summary}[theorem]{Summary}
\newenvironment{proof}[1][Proof]{\noindent\textbf{#1.} }{\ \rule{0.5em}{0.5em}}
\input{tcilatex}
\begin{document}


We are given the following vectors%
\begin{eqnarray*}
\bar{p} &=&\left[ 
\begin{array}{ccc}
\bar{p}_{1} & \bar{p}_{2} & \bar{p}_{3}%
\end{array}%
\right] =\left[ 
\begin{array}{ccc}
9.3 & 5.6 & 4.2%
\end{array}%
\right] \\
c &=&\left[ 
\begin{array}{ccc}
c_{1} & c_{2} & c_{3}%
\end{array}%
\right] =\left[ 
\begin{array}{ccc}
7.8 & c_{2} & c_{3}%
\end{array}%
\right] \\
b &=&\left[ 
\begin{array}{ccc}
b_{1} & b_{2} & b_{3}%
\end{array}%
\right] =\left[ 
\begin{array}{ccc}
b_{1} & b_{2} & 1.04%
\end{array}%
\right] \\
assets &=&\left[ 
\begin{array}{ccc}
a_{1} & a_{2} & a_{3}%
\end{array}%
\right] =\left[ 
\begin{array}{ccc}
9.5 & 6.4 & 4.3%
\end{array}%
\right]
\end{eqnarray*}%
For the vector $c$, we don't know $c_{2}$ and $c_{3}$. For the vector $b$,
we don't know $b_{1}$ and $b_{2}$.

We are also given a matrix $A$ 
\[
A=\left[ 
\begin{array}{ccc}
0 & a_{12} & a_{13} \\ 
a_{21} & 0 & a_{23} \\ 
a_{31} & a_{32} & 0%
\end{array}%
\right] 
\]%
where the diagonal has zeros, and the entries $a_{12}$, $a_{13}$, $a_{21}$, $%
a_{23}$, $a_{31}$, $a_{32}$ are unknown.

We are also given a random vector $x$%
\[
x=\left[ 
\begin{array}{ccc}
x_{1} & x_{2} & x_{3}%
\end{array}%
\right] 
\]%
where each component is drawn from an independent uniform distribution
between 0 and 1:%
\begin{eqnarray*}
x_{1} &\sim &U\left( 0,1\right) \\
x_{2} &\sim &U\left( 0,1\right) \\
x_{3} &\sim &U\left( 0,1\right)
\end{eqnarray*}

We want to solve the following maximization problem. Maximize\ 
\[
\mathbb{E}\left[ \sum_{i=1}^{N}\left( x_{i}-p_{i}\left( x\right) \right) %
\right] 
\]%
subject to the following constraints:

\begin{enumerate}
\item \textquotedblleft Box\textquotedblright\ or bound constraints%
\begin{eqnarray*}
0 &\leq &p_{i}\leq \bar{p}_{i}\text{, }i=1,..,N \\
0 &\leq &c_{i}\leq assets_{i}\text{, }i=1,..,N \\
0 &\leq &b_{i}\leq \bar{p}_{i}\text{, }i=1,..,N \\
0 &\leq &a_{ij}\leq 1\text{, }i,j=1,..,N
\end{eqnarray*}

\item Linear constraints%
\begin{eqnarray*}
\bar{p}_{i}\sum_{j=1}^{N}a_{ij} &=&\bar{p}_{i}-b_{i}\text{, }i=1,..,N \\
\sum_{j=1}^{N}a_{ji}\bar{p}_{j} &=&assets_{i}-c_{i}\text{, }i=1,..,N
\end{eqnarray*}

\item Complementarity constraints%
\begin{eqnarray*}
a_{ii} &=&0\text{, }i=1,..,N \\
a_{ij}a_{ji} &=&0\text{ for }i,j=1...,N\text{ or }\sum_{i=1}^{N}\sum_{j\leq
i}a_{ij}a_{ji}=0
\end{eqnarray*}

\item Non-linear constraints%
\[
p_{i}\left( x\right) =\min \left\{ \bar{p}_{i},\max \left\{ \left( 1+\gamma
\right) \left( \sum_{j=1}^{n}a_{ji}p_{j}\left( x\right) +c_{i}-x_{i}\right)
-\gamma \bar{p}_{i},0\right\} \right\} ,i=1,..,N 
\]
\end{enumerate}

\begin{eqnarray*}
\beta _{i} &=&\frac{\log \left( \delta _{i}\right) }{\log \left( 1-\frac{%
w_{i}}{c_{i}}\right) } \\
\delta _{i} &=&\left( 1-\frac{w_{i}}{c_{i}}\right) ^{\beta _{i}} \\
x_{i} &=&F^{-1}\left( u_{i}\right) \\
&=&-\left( 1-u_{i}\right) ^{\frac{\log \left( 1-\frac{w_{i}}{c_{i}}\right) }{%
\log \left( \delta _{i}\right) }}\log \left( 1-u_{i}\right) \frac{1}{\left(
c_{i}-w_{i}\right) \log \left( \delta _{i}\right) }\frac{w_{i}}{c_{i}} \\
&&
\end{eqnarray*}%
\begin{eqnarray*}
&&\int \left( x_{i}-p_{i}\left( x\right) \right) dF \\
&&\int \left( u_{i}-p_{i}\left( u\right) \right) dF
\end{eqnarray*}

\section{Jacobian of Constraints}

\begin{enumerate}
\item 
\begin{eqnarray*}
&&\bar{p}_{i}\sum_{j=1}^{N}a_{ij}-\bar{p}_{i}+b_{i} \\
&&\sum_{j=1}^{N}a_{ji}\bar{p}_{j}-assets_{i}+c_{i}
\end{eqnarray*}%
\begin{eqnarray*}
\frac{\partial }{\partial a_{ij}}\left[ \bar{p}_{i}\sum_{q=1}^{N}a_{iq}-\bar{%
p}_{i}+b_{i}\right] &=&\bar{p}_{i} \\
\frac{\partial }{\partial b_{i}}\left[ \bar{p}_{i}\sum_{j=1}^{N}a_{ij}-\bar{p%
}_{i}+b_{i}\right] &=&1 \\
\frac{\partial }{\partial c_{i}}\left[ \bar{p}_{i}\sum_{j=1}^{N}a_{ij}-\bar{p%
}_{i}+b_{i}\right] &=&0
\end{eqnarray*}%
\begin{eqnarray*}
\frac{\partial }{\partial a_{ij}}\left[ \sum_{j=1}^{N}a_{ji}\bar{p}%
_{j}-assets_{i}+c_{i}\right] &=&\frac{\partial }{\partial A}\left[ A^{T}\bar{%
p}-assets-c\right] =\bar{p} \\
\frac{\partial }{\partial b_{i}}\left[ \sum_{j=1}^{N}a_{ji}\bar{p}%
_{j}-assets_{i}+c_{i}\right] &=&0 \\
\frac{\partial }{\partial c_{i}}\left[ \sum_{j=1}^{N}a_{ji}\bar{p}%
_{j}-assets_{i}+c_{i}\right] &=&1
\end{eqnarray*}

\item Complementarity constraints%
\begin{eqnarray*}
\frac{\partial }{\partial a_{ij}}\sum_{i=1}^{N}\sum_{j\leq i}a_{ij}a_{ji}
&=&a_{ji}=A^{T} \\
0 &=&a_{11}^{2}+a_{12}a_{21}+a_{13}a_{31}+a_{22}^{2}+a_{23}a_{32}+a_{33}^{2}
\end{eqnarray*}%
\begin{eqnarray*}
&&a_{13} \\
&&%
\begin{array}{c}
a_{11} \\ 
a_{21} \\ 
a_{31} \\ 
a_{12} \\ 
a_{22} \\ 
a_{32} \\ 
a_{13} \\ 
a_{23} \\ 
a_{33}%
\end{array}%
\begin{array}{ccccccccc}
2 &  &  &  &  &  &  &  &  \\ 
&  &  & 1 &  &  &  &  &  \\ 
&  &  &  &  &  & 1 &  &  \\ 
& 1 &  &  &  &  &  &  &  \\ 
&  &  &  & 2 &  &  &  &  \\ 
&  &  &  &  &  &  & 1 &  \\ 
&  & 1 &  &  &  &  &  &  \\ 
&  &  &  &  & 1 &  &  &  \\ 
&  &  &  &  &  &  &  & 2%
\end{array}%
\end{eqnarray*}
\end{enumerate}

\section{SGD}

\[
\mathbb{E}\left[ \sum_{i=1}^{N}\left( -p_{i}\left( x\right) \right) \right] =%
\mathbb{E}_{x}\left[ 1_{N}p\left( x\right) \right] =\int_{\left[ 0,1\right]
^{N}}1_{N}p\left( x\right) F\left( x\right) dx 
\]%
subject to

\begin{enumerate}
\item \textquotedblleft Box\textquotedblright\ or bound constraints%
\begin{eqnarray*}
0 &\leq &p_{i}\leq \bar{p}_{i}\text{, }i=1,..,N \\
0 &\leq &c_{i}\leq assets_{i}\text{, }i=1,..,N \\
0 &\leq &b_{i}\leq \bar{p}_{i}\text{, }i=1,..,N \\
0 &\leq &a_{ij}\leq 1\text{, }i,j=1,..,N
\end{eqnarray*}

\item Linear constraints%
\begin{eqnarray*}
b_{i} &=&\bar{p}_{i}-\bar{p}_{i}\sum_{j=1}^{N}a_{ij}\text{, }i=1,..,N \\
c_{i} &=&assets_{i}-\sum_{j=1}^{N}a_{ji}\bar{p}_{j}\text{, }i=1,..,N
\end{eqnarray*}%
\begin{eqnarray*}
b-\bar{p}+\bar{p}^{T}A1_{N} &=&0 \\
c &=&assets-A^{T}\bar{p}
\end{eqnarray*}%
\begin{eqnarray*}
0 &\leq &b_{i}\leq \bar{p}_{i}\text{ and }b_{i}=\bar{p}_{i}-\bar{p}%
_{i}\sum_{j=1}^{N}a_{ij}\text{ give }0_{N}\leq A1_{N}\leq 1_{N} \\
0 &\leq &c_{i}\leq assets_{i}\text{ and }c_{i}=assets_{i}-%
\sum_{j=1}^{N}a_{ji}\bar{p}_{j}\text{ give }0_{N}\leq A^{T}\left( \bar{p}%
./assets\right) \leq 1_{N} \\
\text{and we know }\frac{\bar{p}}{assets} &\leq &1
\end{eqnarray*}

\item Complementarity constraints%
\begin{eqnarray*}
a_{ii} &=&0\text{, }i=1,..,N \\
a_{ij}a_{ji} &=&0\text{ for }i,j=1...,N\text{ or }\sum_{i=1}^{N}\sum_{j\leq
i}a_{ij}a_{ji}=0 \\
&&vec\left( A\right) ^{T}Mvec\left( A\right) \\
0 &=&a_{12}a_{21}+a_{13}a_{31}+a_{23}a_{32}
\end{eqnarray*}

\item Non-linear constraints%
\begin{eqnarray*}
p_{i}\left( x\right) &=&\min \left\{ \bar{p}_{i},\max \left\{ \left(
1+\gamma \right) \left( \sum_{j=1}^{n}a_{ji}p_{j}\left( x\right)
+c_{i}-x_{i}\right) -\gamma \bar{p}_{i},0\right\} \right\} ,i=1,..,N \\
p\left( x\right) &=&\min \left\{ \bar{p},\max \left\{ \left( 1+\gamma
\right) \left( A^{T}p\left( x\right) +c-x\right) -\gamma \bar{p},0\right\}
\right\} \\
p\left( x\right) &=&\min \left\{ \bar{p},\max \left\{ \left( 1+\gamma
\right) \left( A^{T}p\left( x\right) -A^{T}\bar{p}+assets-x\right) -\gamma 
\bar{p},0\right\} \right\}
\end{eqnarray*}%
\begin{eqnarray*}
\left( 1+\gamma \right) \left( A^{T}p\left( x\right) +c-x\right) -\gamma 
\bar{p} &<&0 \\
A^{T}p\left( x\right) &<&\frac{\gamma }{1+\gamma }\bar{p}-\left( c-x\right)
\\
\frac{\bar{p}}{c} &>&\left( \frac{1}{\gamma }+1\right) \left( 1-x\right)
\end{eqnarray*}
\end{enumerate}

\begin{eqnarray*}
f_{i} &=&\frac{x^{\alpha _{i}-1}\left( 1-x\right) ^{\beta _{i}-1}}{B\left(
\alpha _{i},\beta _{i}\right) } \\
\alpha _{i} &=&1\text{ and }\beta _{i}=\frac{\log \left( \delta _{i}\right) 
}{\log \left( 1-\frac{w_{i}}{c_{i}}\right) } \\
f_{i} &=&\frac{\left( 1-x\right) ^{\frac{\log \left( \delta _{i}\right) }{%
\log \left( 1-\frac{w_{i}}{c_{i}}\right) }-1}}{B\left( 1,\beta _{i}\right) }
\\
\delta _{i} &=&\left( 1-\frac{w_{i}}{c_{i}}\right) ^{\beta _{i}} \\
x_{i} &=&F^{-1}\left( u_{i}\right) \\
&=&-\left( 1-u_{i}\right) ^{\frac{\log \left( 1-\frac{w_{i}}{c_{i}}\right) }{%
\log \left( \delta _{i}\right) }}\log \left( 1-u_{i}\right) \frac{1}{\left(
c_{i}-w_{i}\right) \log \left( \delta _{i}\right) }\frac{w_{i}}{c_{i}}
\end{eqnarray*}%
\[
E\left[ g\left( X_{1},...,X_{d}\right) \right] =\int g\left(
x_{1},...,x_{d}\right) c\left( F_{1}\left( x_{1}\right) ,...,F_{d}\left(
x_{d}\right) \right) f_{1}\left( x_{1}\right) ...f_{d}\left( x_{d}\right)
dx_{1}...dx_{d} 
\]%
\begin{eqnarray*}
&&\min_{a}\mathbb{E}_{x}\left[ 1_{N}p\left( x\right) \right] \\
&&s.t. \\
0 &=&a^{T}Ma
\end{eqnarray*}%
\begin{eqnarray*}
&&\text{Method of multipliers} \\
L_{\rho }\left( a,\lambda \right) &=&\mathbb{E}_{x}\left[ 1_{N}p\left(
x\right) \right] +\lambda a^{T}Ma+\frac{\rho }{2}\left\Vert
a^{T}Ma\right\Vert _{2}^{2} \\
a^{k+1} &=&\arg \min_{a}L_{\rho }\left( a,\lambda ^{k}\right) \\
\lambda ^{k+1} &=&\lambda ^{k}+\rho \left( a^{k+1}\right) ^{T}Ma^{k+1} \\
&&or \\
\hat{L}_{\rho }\left( a,\lambda \right) &=&\mathbb{E}_{x}\left[ 1_{N}p\left(
x\right) \right] +\frac{\rho }{2}\left\Vert a^{T}Ma+u\right\Vert
_{2}^{2}+const \\
a^{k+1} &=&\arg \min_{a}\hat{L}_{\rho }\left( a,\lambda ^{k}\right) \\
u^{k+1} &=&u^{k}+a^{T}Ma
\end{eqnarray*}%
\begin{eqnarray*}
&&\text{ADMM} \\
&&\min_{a}\mathbb{E}_{x}\left[ 1_{N}p\left( x\right) \right] +g\left(
z\right) \\
a-z &=&0 \\
g\left( z\right) &=&\mathbf{1}\left\{ 0=z^{T}Mz\right\} \\
a^{k+1} &=&\arg \min_{a}\mathbb{E}_{x}\left[ 1_{N}p\left( x\right) \right] +%
\frac{\rho }{2}\left\Vert a-z^{k}+u^{k}\right\Vert _{2}^{2} \\
z^{k+1} &=&\Pi _{\left\{ 0=z^{T}Mz\right\} }\left( a^{k+1}+u^{k}\right) \\
u^{k+1} &=&u^{k}+a^{k+1}-z^{k+1} \\
\Pi _{\left\{ 0=z^{T}Mz\right\} }\left( v\right) &=&\arg \min_{z}\left\{ 
\mathbf{1}\left\{ 0=z^{T}Mz\right\} +\frac{\rho }{2}\left\Vert
z-v\right\Vert _{2}^{2}\right\} =prox_{g,\rho }\left( v\right) \\
\Pi _{\left\{ 0=z^{T}Mz\right\} }\left( a^{k+1}+u^{k}\right) &=&\arg
\min_{z}\left\{ \mathbf{1}\left\{ 0=z^{T}Mz\right\} +\frac{\rho }{2}%
\left\Vert z-a^{k+1}-u^{k}\right\Vert _{2}^{2}\right\} =prox_{g,\rho }\left(
a^{k+1}+u^{k}\right)
\end{eqnarray*}

\begin{eqnarray*}
&&\text{Consensus optimization} \\
&&\min_{a}\mathbb{E}_{x}\left[ \sum_{i=1}^{N}p_{i}\left( x\right) \right]
+g\left( z\right)  \\
a-z &=&0 \\
g\left( z\right)  &=&\mathbf{1}\left\{ 0=z^{T}Mz\right\}  \\
a^{k+1} &=&\arg \min_{a}\mathbb{E}_{x}\left[ 1_{N}p\left( x\right) \right] +%
\frac{\rho }{2}\left\Vert a-z^{k}+u^{k}\right\Vert _{2}^{2} \\
z^{k+1} &=&\Pi _{\left\{ 0=z^{T}Mz\right\} }\left( a^{k+1}+u^{k}\right)  \\
u^{k+1} &=&u^{k}+a^{k+1}-z^{k+1} \\
\Pi _{\left\{ 0=z^{T}Mz\right\} }\left( v\right)  &=&\arg \min_{z}\left\{ 
\mathbf{1}\left\{ 0=z^{T}Mz\right\} +\frac{\rho }{2}\left\Vert
z-v\right\Vert _{2}^{2}\right\} =prox_{g,\rho }\left( v\right)  \\
\Pi _{\left\{ 0=z^{T}Mz\right\} }\left( a^{k+1}+u^{k}\right)  &=&\arg
\min_{z}\left\{ \mathbf{1}\left\{ 0=z^{T}Mz\right\} +\frac{\rho }{2}%
\left\Vert z-a^{k+1}-u^{k}\right\Vert _{2}^{2}\right\} =prox_{g,\rho }\left(
a^{k+1}+u^{k}\right) 
\end{eqnarray*}%
\begin{eqnarray*}
&&\int \left( x_{i}-p_{i}\left( x\right) \right) dF \\
&&\int \left( u_{i}-p_{i}\left( u\right) \right) dF
\end{eqnarray*}%
\begin{eqnarray*}
&&%
\begin{array}{c}
a_{11} \\ 
a_{21} \\ 
a_{12} \\ 
a_{22}%
\end{array}%
^{T}\left[ 
\begin{array}{cccc}
M_{11} & M_{12} & M_{13} & M_{14} \\ 
M_{21} & M_{22} & M_{23} & M_{24} \\ 
M_{31} & M_{32} & M_{33} & M_{34} \\ 
M_{41} & M_{42} & M_{43} & M_{44}%
\end{array}%
\right] 
\begin{array}{c}
a_{11} \\ 
a_{21} \\ 
a_{12} \\ 
a_{22}%
\end{array}
\\
&&a_{11},a_{21},a_{12},a_{22} \\
&&\left[ 
\begin{array}{ccc}
a_{11} & a_{12} & a_{13} \\ 
a_{21} & a_{22} & a_{23} \\ 
a_{31} & a_{32} & a_{33}%
\end{array}%
\right] ^{T}\left[ 
\begin{array}{ccc}
a_{11} & a_{12} & a_{13} \\ 
a_{21} & a_{22} & a_{23} \\ 
a_{31} & a_{32} & a_{33}%
\end{array}%
\right] 
\end{eqnarray*}%
\[
a_{11}\left( M_{11}a_{11}+M_{21}a_{21}+M_{31}a_{12}+M_{41}a_{22}\right)
+a_{21}\left( M_{12}a_{11}+M_{22}a_{21}+M_{32}a_{12}+M_{42}a_{22}\right)
+a_{12}\left( M_{13}a_{11}+M_{23}a_{21}+M_{33}a_{12}+M_{43}a_{22}\right)
+a_{22}\left( M_{14}a_{11}+M_{24}a_{21}+M_{34}a_{12}+M_{44}a_{22}\right) 
\]%
$=\allowbreak $%
\[
\frac{1}{2}%
\begin{array}{c}
a_{11} \\ 
a_{21} \\ 
a_{12} \\ 
a_{22}%
\end{array}%
^{T}\left[ 
\begin{array}{cccc}
2 & 0 & 0 & 0 \\ 
0 & 0 & 1 & 0 \\ 
0 & 1 & 0 & 0 \\ 
0 & 0 & 0 & 2%
\end{array}%
\right] 
\begin{array}{c}
a_{11} \\ 
a_{21} \\ 
a_{12} \\ 
a_{22}%
\end{array}%
\]%
\begin{eqnarray*}
&&M_{11}a_{11}^{2}+a_{21}a_{12}+M_{44}a_{22}^{2} \\
1 &=&M_{11} \\
1 &=&M_{44} \\
1 &=&M_{23}+M_{32} \\
0 &=&M_{12}+M_{21} \\
0 &=&M_{13}+M_{31} \\
0 &=&M_{14}+M_{41} \\
0 &=&M_{22} \\
0 &=&M_{24}+M_{42} \\
0 &=&M_{33} \\
0 &=&M_{34}+M_{43}
\end{eqnarray*}%
$\allowbreak $%
\begin{eqnarray*}
p\left( x\right)  &=&\min \left\{ \bar{p},\max \left\{ A^{T}p\left( x\right)
-A^{T}\bar{p}+assets-cx,0\right\} \right\}  \\
p\left( x\right)  &=&\min \left\{ \bar{p},\max \left\{ A^{T}\min \left\{
0,assets-\bar{p}-cx\right\} +assets-cx,0\right\} \right\}  \\
p\left( x\right)  &=&\min \left\{ \bar{p},\max \left\{ A^{T}\min \left\{
0,assets-\bar{p}-cx\right\} +assets-cx,0\right\} \right\} 
\end{eqnarray*}%
\begin{eqnarray*}
\bar{p} &\leq &assets \\
w &=&assets-\bar{p}
\end{eqnarray*}%
\begin{eqnarray*}
\min \left\{ \bar{p},assets-cx\right\} -\bar{p} &=&\bar{p}-\bar{p}=0 \\
\min \left\{ \bar{p},assets-cx\right\} -\bar{p} &=&assets-cx-\bar{p}
\end{eqnarray*}%
\[
\min \left\{ 0,assets-cx-\bar{p}\right\} 
\]%
\begin{eqnarray*}
A &=&\left[ 
\begin{array}{cc}
a_{11} & a_{12} \\ 
a_{21} & a_{22}%
\end{array}%
\right] ,A^{T}=\left[ 
\begin{array}{cc}
a_{11} & a_{21} \\ 
a_{12} & a_{22}%
\end{array}%
\right] ,p=\left[ 
\begin{array}{c}
p_{1} \\ 
p_{2}%
\end{array}%
\right] ,\bar{p}=\left[ 
\begin{array}{c}
\bar{p}_{1} \\ 
\bar{p}_{2}%
\end{array}%
\right] ,assets=\left[ 
\begin{array}{c}
assets_{1} \\ 
assets_{2}%
\end{array}%
\right] ,cx=\left[ 
\begin{array}{c}
c_{1}x_{1} \\ 
c_{2}x_{2}%
\end{array}%
\right]  \\
A^{T}p\left( x\right) -A^{T}\bar{p}+assets-cx &=&\left[ 
\begin{array}{c}
p_{1}a_{11}+p_{2}a_{21} \\ 
p_{1}a_{12}+p_{2}a_{22}%
\end{array}%
\right] -\left[ 
\begin{array}{c}
\bar{p}_{1}a_{11}+\bar{p}_{2}a_{21} \\ 
\bar{p}_{1}a_{12}+\bar{p}_{2}a_{22}%
\end{array}%
\right] +\left[ 
\begin{array}{c}
assets_{1} \\ 
assets_{2}%
\end{array}%
\right] -\left[ 
\begin{array}{c}
c_{1}x_{1} \\ 
c_{2}x_{2}%
\end{array}%
\right]  \\
&=&\left[ 
\begin{array}{c}
p_{1}a_{11}+p_{2}a_{21}-\left( \bar{p}_{1}a_{11}+\bar{p}_{2}a_{21}\right)
+assets_{1}-c_{1}x_{1} \\ 
p_{1}a_{12}+p_{2}a_{22}-\left( \bar{p}_{1}a_{12}+\bar{p}_{2}a_{22}\right)
+assets_{2}-c_{2}x_{2}%
\end{array}%
\right]  \\
\max \left\{ A^{T}p\left( x\right) -A^{T}\bar{p}+assets-cx,0\right\}  &=&%
\left[ 
\begin{array}{c}
\max \left\{ p_{1}a_{11}+p_{2}a_{21}-\left( \bar{p}_{1}a_{11}+\bar{p}%
_{2}a_{21}\right) +assets_{1}-c_{1}x_{1},0\right\}  \\ 
\max \left\{ p_{1}a_{12}+p_{2}a_{22}-\left( \bar{p}_{1}a_{12}+\bar{p}%
_{2}a_{22}\right) +assets_{2}-c_{2}x_{2},0\right\} 
\end{array}%
\right]  \\
\min \left\{ \bar{p},\max \left\{ A^{T}p\left( x\right) -A^{T}\bar{p}%
+assets-cx,0\right\} \right\}  &=&\left[ 
\begin{array}{c}
\min \left\{ \bar{p}_{1},\max \left\{ p_{1}a_{11}+p_{2}a_{21}-\left( \bar{p}%
_{1}a_{11}+\bar{p}_{2}a_{21}\right) +assets_{1}-c_{1}x_{1},0\right\}
\right\}  \\ 
\min \left\{ \bar{p}_{2},\max \left\{ p_{1}a_{12}+p_{2}a_{22}-\left( \bar{p}%
_{1}a_{12}+\bar{p}_{2}a_{22}\right) +assets_{2}-c_{2}x_{2},0\right\}
\right\} 
\end{array}%
\right]  \\
p_{0}\left( x\right)  &=&\min \left\{ \bar{p},\max \left\{
assets-cx,0\right\} \right\} =\left[ 
\begin{array}{c}
\min \left\{ \bar{p}_{1},\max \left\{ assets_{1}-c_{1}x_{1},0\right\}
\right\}  \\ 
\min \left\{ \bar{p}_{2},\max \left\{ assets_{2}-c_{2}x_{2},0\right\}
\right\} 
\end{array}%
\right]  \\
p_{1}\left( x\right)  &=&\min \left\{ \bar{p},\max \left\{ A^{T}p_{0}\left(
x\right) -A^{T}\bar{p}+assets-cx,0\right\} \right\}  \\
&=&\left[ 
\begin{array}{c}
\min \left\{ \bar{p}_{1},\max \left\{ \min \left\{ \bar{p}_{1},\max \left\{
assets_{1}-c_{1}x_{1},0\right\} \right\} a_{11}+\min \left\{ \bar{p}%
_{2},\max \left\{ assets_{2}-c_{2}x_{2},0\right\} \right\} a_{21}-\left( 
\bar{p}_{1}a_{11}+\bar{p}_{2}a_{21}\right) +assets_{1}-c_{1}x_{1},0\right\}
\right\}  \\ 
\min \left\{ \bar{p}_{2},\max \left\{ \min \left\{ \bar{p}_{1},\max \left\{
assets_{1}-c_{1}x_{1},0\right\} \right\} a_{12}+\min \left\{ \bar{p}%
_{2},\max \left\{ assets_{2}-c_{2}x_{2},0\right\} \right\} a_{22}-\left( 
\bar{p}_{1}a_{12}+\bar{p}_{2}a_{22}\right) +assets_{2}-c_{2}x_{2},0\right\}
\right\} 
\end{array}%
\right] 
\end{eqnarray*}%
\begin{eqnarray*}
y &=&\min \left\{ U,\max \left\{ x,L\right\} \right\}  \\
&=&\max \left\{ L,x\right\} -\max \left\{ x,U,L\right\} +U \\
&=&\max \left\{ L,x\right\} -\max \left\{ U,x\right\} +U \\
&=&x+\max \left\{ L-x,0\right\} -\max \left\{ x-U,0\right\} 
\end{eqnarray*}%
\begin{eqnarray*}
&&\frac{1}{2}%
\begin{array}{c}
a_{11} \\ 
a_{21} \\ 
a_{12} \\ 
a_{22}%
\end{array}%
^{T}\left[ 
\begin{array}{cccc}
2 & 0 & 0 & 0 \\ 
0 & 0 & 1 & 0 \\ 
0 & 1 & 0 & 0 \\ 
0 & 0 & 0 & 2%
\end{array}%
\right] 
\begin{array}{c}
a_{11} \\ 
a_{21} \\ 
a_{12} \\ 
a_{22}%
\end{array}
\\
&&\frac{1}{2}%
\begin{array}{c}
a_{21} \\ 
a_{12}%
\end{array}%
^{T}\left[ 
\begin{array}{cc}
0 & 1 \\ 
1 & 0%
\end{array}%
\right] 
\begin{array}{c}
a_{21} \\ 
a_{12}%
\end{array}%
\end{eqnarray*}%
: $2a_{12}a_{21}$ 
\[
\begin{array}{ccccccccc}
2 &  &  &  &  &  &  &  &  \\ 
&  &  & 1 &  &  &  &  &  \\ 
&  &  &  &  &  & 1 &  &  \\ 
& 1 &  &  &  &  &  &  &  \\ 
&  &  &  & 2 &  &  &  &  \\ 
&  &  &  &  &  &  & 1 &  \\ 
&  & 1 &  &  &  &  &  &  \\ 
&  &  &  &  & 1 &  &  &  \\ 
&  &  &  &  &  &  &  & 2%
\end{array}%
\]%
$%
\begin{array}{cccccc}
&  & 1 &  &  &  \\ 
&  &  &  & 1 &  \\ 
1 &  &  &  &  &  \\ 
&  &  &  &  & 1 \\ 
& 1 &  &  &  &  \\ 
&  &  & 1 &  & 
\end{array}%
$%
\begin{eqnarray*}
&&\left\{ \left( t,x\right) \in R^{d}:\left\Vert x\right\Vert _{2}\leq
t\right\}  \\
&&\left\{ \left( t,u,x\right) \in R^{d}:\left\Vert x\right\Vert _{2}\leq
t\right\}  \\
a_{12}a_{21} &=&0 \\
\begin{array}{c}
a_{12} \\ 
a_{21}%
\end{array}
&=&%
\begin{array}{cc}
\frac{1}{\sqrt{2}} & \frac{1}{\sqrt{2}} \\ 
\frac{1}{\sqrt{2}} & -\frac{1}{\sqrt{2}}%
\end{array}%
\begin{array}{c}
x_{12} \\ 
x_{21}%
\end{array}%
=%
\begin{array}{c}
\frac{1}{\sqrt{2}}\left( x_{12}+x_{21}\right)  \\ 
\frac{1}{\sqrt{2}}\left( x_{12}-x_{21}\right) 
\end{array}
\\
\begin{array}{c}
x_{12} \\ 
x_{21}%
\end{array}
&=&%
\begin{array}{cc}
\frac{1}{\sqrt{2}} & \frac{1}{\sqrt{2}} \\ 
\frac{1}{\sqrt{2}} & -\frac{1}{\sqrt{2}}%
\end{array}%
^{-1}%
\begin{array}{c}
a_{12} \\ 
a_{21}%
\end{array}%
=%
\begin{array}{c}
\frac{1}{\sqrt{2}}\left( a_{12}+a_{21}\right)  \\ 
\frac{1}{\sqrt{2}}\left( a_{12}-a_{21}\right) 
\end{array}
\\
a_{12},a_{21} &\geq &0,2a_{12}a_{21}=0 \\
&\Longrightarrow &x_{12}^{2}-x_{21}^{2}=0,x_{12}\geq 0 \\
x_{12}^{2} &\geq &x_{21}^{2},x_{12}\geq 0 \\
&\Longrightarrow &2a_{12}a_{21}=0,a_{12},a_{21}\geq 0 \\
&&\left\{ \left( t,x\right) \in R^{d}:\left\Vert x\right\Vert _{2}\leq
t\right\}  \\
\left\Vert x_{12}\right\Vert _{2} &\geq &x_{21},x_{12}\geq
0,t=1,u=x_{21},x=x_{12}
\end{eqnarray*}%
$\allowbreak $%
\begin{eqnarray*}
2a_{12}a_{21} &\geq &0 \\
a_{12},a_{21} &\geq &0
\end{eqnarray*}%
\[
x_{12}\geq \left\Vert x_{12}\right\Vert _{2},x_{12}\geq 0
\]%
\[
\left\vert x\right\vert \leq t\iff \left( t,x\right) \in Q^{2}
\]%
\[
\left[ 
\begin{array}{c}
b_{1} \\ 
b_{2}%
\end{array}%
\right] ^{T}\left[ 
\begin{array}{cc}
0 & a_{12} \\ 
a_{21} & 0%
\end{array}%
\right] \left[ 
\begin{array}{c}
b_{3} \\ 
b_{4}%
\end{array}%
\right] =b_{1}b_{2}a_{21}+b_{2}b_{1}a_{12}
\]%
: $b_{1}b_{4}a_{12}+b_{2}b_{3}a_{21}$ : :%
\[
\begin{array}{c}
a_{11} \\ 
a_{21} \\ 
a_{12} \\ 
a_{22}%
\end{array}%
\begin{array}{c}
a_{11} \\ 
a_{21} \\ 
a_{12} \\ 
a_{22}%
\end{array}%
^{T}
\]
: $%
\begin{array}{cccc}
a_{11}^{2} & a_{11}a_{21} & a_{11}a_{12} & a_{11}a_{22} \\ 
a_{11}a_{21} & a_{21}^{2} & a_{12}a_{21} & a_{21}a_{22} \\ 
a_{11}a_{12} & a_{12}a_{21} & a_{12}^{2} & a_{12}a_{22} \\ 
a_{11}a_{22} & a_{21}a_{22} & a_{12}a_{22} & a_{22}^{2}%
\end{array}%
\allowbreak $

\end{document}
